theories/Interp/Network.v
@@ -1,6 +1,7 @@
 From Coq Require Import
      Fin
      Nat
+     List
      Relations.
 
 From Equations Require Import Equations.
@@ -14,6 +15,7 @@ From CTree Require Import
      CTree
      Equ
      SBisim
+     Misc.Vectors
      Core.Utils.
 
 From ExtLib Require Import
@@ -22,94 +24,102 @@ From ExtLib Require Import
 From Coinduction Require Import
      coinduction rel tactics.
 
-From DSL Require Import
-     Vectors
-     Lists
-     Utils
-     Storage
-     Log
-     System.
-
-Import MonadNotation ListNotations EquNotations SBisimNotations Log.
+Import MonadNotation.
+Import ListNotations.
+Import EquNotations.
 Local Open Scope monad_scope.
 Local Open Scope fin_vector_scope.
 
-
 Set Implicit Arguments.
 
-Module Network(S: Systems).
-  Module StorageM := Storage(S).
-  Import StorageM S.
+Module Network.
 
-  Section ParametricN.
-    Variable (n: nat).
-
-    (** Messages exchagend *)
+  (*| IP addresses |*)
+  Notation uid := fin.
+  
+  Section Messaging.
+    (*| [n] number of processes
+        [msg] type of messages |*)
+    Context (n: nat) (msg: Set) {E C: Type -> Type} {HasStuck: B0 -< C}.
+    
+    (*| Messages exchagend |*)
     Record req := {
         principal: uid n;
         payload: msg;
       }.
 
-    (** A queue of messages *)
+    (*| A queue of messages |*)
     Definition queue := list req.
 
-    (** Network effects *)
+    (*| Network effects |*)
     Inductive Net: Type -> Type :=
     | Recv: Net (option req)
     | Send : req -> Net unit
     | Broadcast: msg -> Net unit.
     
-    (** A task is either running or returned *)
-    Inductive Task (E: Type -> Type) :=
-    | Running (c: ctree E void)(q: queue)
-    | Blocked (k: option req -> ctree E void).
-    (** this is a "soft" blocked -- the scheduler can pass it "None"
+    (*| A task is either running or returned |*)
+    Inductive Task :=
+    | Running (c: ctree E C void)(q: queue)
+    (** this is "soft" blocked -- the scheduler can pass it "None"
         which corresponds to a timeout, and it will unblock *)
+    | Blocked (k: option req -> ctree E C void).
+    
+  End Messaging.
 
-  End ParametricN.
-
-  Arguments Running {n} {E}.
-  Arguments Blocked {n} {E}.
-  Arguments Send {n}.
-  Arguments Recv {n}.
-  Arguments Broadcast {n}.
-
-  Definition recv {n E} `{Net n -< E}: ctree E (option (req n)) := trigger Recv.
-  Definition send {n E} `{Net n -< E}: uid n -> msg -> ctree E unit :=
+  (*| API for messaging processes |*)
+  Arguments Running {n} {msg} {E C}.
+  Arguments Blocked {n} {msg} {E C}.
+  Arguments Send {n} {msg}.
+  Arguments Recv {n} {msg}.
+  Arguments Broadcast {n} {msg}.
+  
+  Definition recv {n msg E C} `{Net n msg -< E}: ctree E C (option (req n msg)) := trigger Recv.
+  Definition send {n msg E C} `{Net n msg -< E}: uid n -> msg -> ctree E C unit :=
     fun u p => trigger (Send {| principal := u; payload := p |}).
-  Definition broadcast {n E} `{Net n -< E}: msg -> ctree E unit :=
+  Definition broadcast {n msg E C} `{Net n msg -< E}: msg -> ctree E C unit :=
     fun bs => trigger (Broadcast bs).
 
-  (** A process running forever *)
-  Notation daemon t := (@CTree.forever _ _ void t).
-  
-  Notation Sys n E := (vec n (Task n E)) (only parsing).
+  (*| A process running forever |*)
+  Notation daemon t := (@CTree.forever _ _ _ _ void t).
 
-  (** Unfair but general scheduler *)
-  Equations schedule_one{E: Type -> Type}{n: nat}
-            (schedule: Sys n (Net n +' E) -> ctree E void)
-            (sys: Sys n (Net n +' E)) (r: fin n): ctree E void :=
-    schedule_one schedule sys r with sys $ r => {
-        schedule_one _ _ _ (Running a q) with observe a => {
-          (** A previous choice, traverse it *)
-          schedule_one _ _ _ _ (BrF b n' k) :=
-          Br b n' (fun i' => schedule (sys @ r := Running (k i') q));
-          
-          (** A network `send` effect, interpet it! *)
-          schedule_one _ _ _ _ (VisF (inl1 (Send m)) k) :=
-          let msg' := {| principal := r; payload := payload m |} in
-          let sys' := sys @ r := Running (k tt) q in
-          match sys $ principal m with
-          | Running a' q' =>  
-              (** Deliver to running *)
-              Guard (schedule (sys' @ (principal m) := Running a' (List.cons msg' q')))
-          | Blocked kk => 
-              (** Deliver to blocked processes and unblock them *)
-              Guard (schedule (sys' @ (principal m) := Running (kk (Some msg')) List.nil))
-          end;
+  (*| Contexts -- when a process enters and exits thelet's see how far we go before universe inconsistency |*)
+  Inductive frameE(n: nat): Type -> Type :=
+  | Enter: uid n -> frameE n unit.
 
-          (** Receive a message *)
-          schedule_one _ _ _ _ (VisF (inl1 Recv) k) :=
+  Arguments Enter {n}.
+
+  Definition enter {n E C} `{frameE n -< E} : uid n -> ctree E C unit :=
+    fun u => trigger (Enter u).
+
+  Section Scheduler.
+    Context (n: nat) (msg: Set) {E C: Type -> Type} `{B1 -< C} `{B2 -< C} `{Bn -< C}.
+    Notation Sys := (vec n (@Task n msg (Net n msg +' E) C)) (only parsing).
+
+    (*| General coinductive scheduler |*)
+    Equations schedule_one
+              (schedule: Sys -> ctree (frameE n +' E) C void)
+              (sys: Sys) (r: uid n): ctree (frameE n +' E) C void :=
+      schedule_one schedule sys r with sys $ r => {
+          schedule_one _ _ _ (Running a q) with observe a => {
+            (** A previous choice, traverse it *)
+            schedule_one _ _ _ _ (BrF b c k) :=
+            Br b c (fun i' => schedule (sys @ r := Running (k i') q));
+            
+            (** A network `send` effect, interpet it! *)
+            schedule_one _ _ _ _ (VisF (inl1 (Send m)) k) :=
+            let msg' := {| principal := r; payload := payload m |} in
+            let sys' := sys @ r := Running (k tt) q in
+            match sys $ principal m with
+            | Running a' q' =>  
+                (** Deliver to running *)
+                Guard (schedule (sys' @ (principal m) := Running a' (List.cons msg' q')))
+            | Blocked kk => 
+                (** Deliver to blocked processes and unblock them *)
+                Guard (schedule (sys' @ (principal m) := Running (kk (Some msg')) List.nil))
+            end;
+
+            (** Receive a message *)
+            schedule_one _ _ _ _ (VisF (inl1 Recv) k) :=
             (** Check my inbox q *)
             match last q with
             | Some msg =>
@@ -120,102 +130,80 @@ Module Network(S: Systems).
                 Guard (schedule (sys @ r := Blocked k))
             end;
 
-          (** Broadcast a message to everyone *)
-          schedule_one _ _ _ _ (VisF (inl1 (Broadcast b)) k) :=
+            (** Broadcast a message to everyone *)
+            schedule_one _ _ _ _ (VisF (inl1 (Broadcast b)) k) :=
             let msg := {| principal := r; payload := b |} in
             let sys' := Vector.map (fun a => match a with
-                                   | Running a q => Running a (List.cons msg q)
-                                   | Blocked kk => Running (kk (Some msg)) List.nil
-                                   end) sys in 
+                                          | Running a q => Running a (List.cons msg q)
+                                          | Blocked kk => Running (kk (Some msg)) List.nil
+                                          end) sys in 
             Guard (schedule (sys' @ r := Running (k tt) q));
-          
-          (** Some other downstream effect, trigger *)
-          schedule_one _ _ _ _ (VisF (inr1 e) k) :=
+            
+            (** Some other downstream effect, trigger *)
+            schedule_one _ _ _ _ (VisF (inr1 e) k) :=
             Guard (schedule (sys @ r := Running (trigger e >>= k) q))
-        };
-        (** If the agent is blocked, it could timeout or stay blocked *)
-        schedule_one _ _ _ (Blocked k) :=
-          brD2
-            (schedule (sys @ r := Running (k None) List.nil))  (** Timeout *)
-            (schedule (sys @ r := Blocked k));                 (** Keep blocking *)
-    }.
+          };
+          (** If the agent is blocked, it could timeout or stay blocked *)
+          schedule_one _ _ _ (Blocked k) :=
+            brD2
+              (schedule (sys @ r := Running (k None) List.nil))  (** Timeout *)
+              (schedule (sys @ r := Blocked k));                 (** Keep blocking *)
+        }.
 
-  Import CTree.
-  CoFixpoint schedule{E}{n: nat}(sys: Sys n (Net n +' E)): ctree E void :=
-    r <- br true n ;;
-    schedule_one schedule sys r.
+    CoFixpoint schedule(sys: Sys): ctree (frameE n +' E) C void :=
+      (* Nondterministic pick of a client to run *)
+      r <- branch true (branchn n) ;;
+      (* Mark context switch *)
+      enter r;;
+      (* Schedule it *)
+      schedule_one schedule sys r.
 
-  (** Fair scheduler *)
-  CoFixpoint schedule_fair'{E}{n: nat}(picked: list (fin n))(sys: Sys n (Net n +' E)): ctree E void :=
-    if (length picked =? n) then
-      r <- br true n;;
-      schedule_one (schedule_fair' [r]) sys r
-    else
-      r <- CTree.iter (fun _: unit =>                  
-                        r <- br true n ;;
-                        if (in_dec Fin.eq_dec r picked) then  
-                          ret (inl tt)
-                        else
-                          ret (inr r)) tt;;
-      schedule_one (schedule_fair' (r :: picked)) sys r.
+    (*| Fair scheduler, uses a list of scheduled processes to avoid
+      infinitely rescheduling the same process. |*)
+    CoFixpoint schedule_fair'(picked: list (fin n))(sys: Sys):
+      ctree (frameE n +' E) C void :=
+      if (length picked =? n) then
+        r <- branch true (branchn n);;
+        enter r;;
+        schedule_one (schedule_fair' [r]%list) sys r
+      else
+        r <- CTree.iter (fun _: unit =>                  
+                          r <- branch true (branchn n) ;;
+                          if (in_dec Fin.eq_dec r picked) then  
+                            ret (inl tt)
+                          else
+                            ret (inr r)) tt;;
+        enter r;;
+        schedule_one (schedule_fair' (r :: picked)) sys r.
 
-  Notation schedule_fair := (schedule_fair' []%list) (only parsing).
-                                                              
-  Transparent schedule.
-  Transparent schedule_fair'.
-  Transparent schedule_one.
-  Transparent vector_replace.
+    Notation schedule_fair := (schedule_fair' []%list) (only parsing).
+    
+    Transparent schedule.
+    Transparent schedule_fair'.
+    Transparent schedule_one.
+    Transparent vector_replace.
 
-  Lemma unfold_schedule{E}{n: nat}(sys: Sys n (Net n +' E)) :
-    schedule sys ≅ (r <- br true n ;; schedule_one schedule sys r).
-  Proof.
-    __step_equ; cbn; econstructor; reflexivity.
-  Qed.    
+    Lemma unfold_schedule(sys: Sys) :
+      schedule sys ≅ (r <- branch true (branchn n) ;; enter r;; schedule_one schedule sys r).
+    Proof.
+      __step_equ; cbn; econstructor; reflexivity.
+    Qed.    
 
-  Import VectorNotations.
-  Lemma unfold_schedule_fair{E}{n: nat}(sys: Sys n (Net n +' E)):
-    n = 0 \/
-      exists (r: fin n) (l: list (fin n)),
-        schedule_fair sys ≅ schedule_one (schedule_fair' (r :: l)) sys r.
-  Proof.    
-    induction n. 
-    - left; reflexivity.
-    - right.
-      unfold schedule_one.
-
-      unfold schedule_fair'; cbn.
-      destruct (inversion_Sn sys) as [h  [ts H]]; subst.
-      exists F1.
-
-      cbn.
+    (** Evaluates Net *)
+    Program Definition run_network(s: vec n (ctree (Net n msg +' E) C void)):
+      ctree (frameE n +' E) C void :=
+      schedule (Vector.map (fun it => Running it List.nil) s).
+    
+    #[global] Instance sbisim_network_goal `{B0 -< C}:
+      Proper (pairwise (sbisim eq) ==> sbisim eq) run_network.
+    Proof.
+      unfold Proper, pairwise, respectful.
+      unfold sbisim.
       coinduction ? CIH.
-    - rewrite (inversion_0 sys); cbn*.
-      simp schedule_one; cbn.
-      
-      cbn.
-      econstructor.
-    unfold schedule_fair'; cbn.
-    simp schedule_one.
-    cbn.
-  (** Evaluates Net *)
-  Program Definition run_network{E n} (s: vec n (ctree (Net n +' E) void)): ctree E void :=
-    schedule (Vector.map (fun it => Running it List.nil) s).
+      intros x y FORALL.
+      unfold run_network.
+      (* TODO: complete *)
+    Admitted.
 
-  
-  #[global] Instance sbisim_network_goal{n E}:
-    Proper (pairwise sbisim ==> sbisim) (@run_network E n).
-  Proof.
-    unfold Proper, pairwise, respectful.
-    unfold sbisim.
-    coinduction ? CIH.
-    intros x y FORALL.
-    unfold run_network.
-
-  Admitted.
-
-  (** ================================================================================ *)
-  (** This is the top-level denotation of a distributed system to a ctree of behaviors *)
-  Program Definition run_storage_network{n}(v: vec n (ctree (Storage +' Net n) void)): heap -> ctree (logE heap) void :=
-    fun st: heap => run_network (Vector.map swap (run_states_log v st)).
+  End Scheduler.
 End Network.
-
