examples/Messaging/Toy.v
@@ -1,0 +1,92 @@
+From ITree Require Import
+     Basics
+     Subevent
+     Indexed.Sum.
+
+From Coq Require Import
+     Fin.
+
+From ExtLib Require Import
+     Monad
+     Option.
+
+From Coinduction Require Import
+     coinduction rel tactics.
+
+From CTree Require Import
+     CTree
+     Interp
+     Interp.State
+     Interp.Log
+     Interp.Network
+     Logic.Ltl
+     Misc.Vectors
+     Eq
+     SBisim.
+
+Import CTreeNotations VectorNotations LtlNotations Monads Log Network.
+
+Local Open Scope fin_vector_scope.
+Local Open Scope ctree_scope.
+
+Set Implicit Arguments.
+Set Maximal Implicit Insertion.
+Set Asymmetric Patterns.
+
+(** ================================================================================ *)
+(** This is the top-level denotation *)
+Program Definition run{n C S} `{B1 -< C} `{B2 -< C} `{Bn -< C}
+        (v: vec n (ctree (Net n S +' stateE S) C void)): S -> ctree (frameE n +' logE S) C void :=
+  fun st: S => run_network (run_states_log v st).
+  
+Module Toy.
+
+  Notation heap := nat. 
+  Notation Net := (Net 2 nat).
+  Notation State := (stateE heap).
+  Notation Sys := (vec 2 (ctree (Net +' State))).
+
+  Section ParametricC.
+    Context {C: Type -> Type} `{B0 -< C} `{B1 -< C} `{B2 -< C} `{Bn -< C}.
+
+    (*| This is a simple two process [a, b] system with a [nat] state.
+
+        For process (i in [a, b]) try to receive a number:
+        - If timeout without receiving, send current state [v] to the other process
+        - If [v] received, store [v] it and send [S v] to the other process 
+    |*)
+    Definition example(them: uid 2): ctree (Net +' State) C void :=
+      daemon (
+          m <- recv ;;
+          match m with
+          | None =>
+              v <- get ;;
+              send them v
+          | Some (Build_req _ v) =>
+              put v ;;
+              send them (S v)
+          end).
+    
+    Program Definition a : uid 2 := @of_nat_lt 0 2 _.
+    Program Definition b : uid 2 := @of_nat_lt 1 2 _.
+
+    Arguments label: clear implicits.
+
+    (*| A context switch event predicate -- process [m] is scheduled *)
+    Variant is_in_frame: uid 2 -> label (frameE 2 +' logE nat) -> Prop :=
+      | ProcessEnter: forall m, is_in_frame m (obs (inl1 (Enter m)) tt).
+
+    Variant is_eq: nat -> label (frameE 2 +' logE nat) -> Prop :=
+      | IsEqualTo: forall n, is_eq n (obs (inr1 (Log n)) tt).
+
+    Lemma liveness: forall i,
+        let sys := run [example b; example a]%vector 0 in
+        sys |= InfinitelyOften (Spec (is_in_frame i)) -> (* Axiomatize fairness *)
+        sys |= Eventually (Spec (is_eq 2)).             (* Process [i] will count to 2 *)
+    Proof.
+      intros i sys Fair.
+      (* WIP *)
+    Admitted.
+  End ParametricC.
+End Toy.
+
